wip

proof/correctness/DistrUtils.ec
@@ -29,3 +29,65 @@ move => l; rewrite supp_dlist // /(\o) /=; move => [??].
 apply Array96.ext_eq => ??.
 by rewrite /get8 initiE // get_of_list //= get_of_list.
 qed.
+
+abstract theory DListProgramX.
+
+type t.
+op d : t distr.
+
+clone import DList.Program 
+with type t <- t,
+     op d <- d.
+
+module SampleX = {
+  proc samplecat(n1 n2: int): t list = {
+   var x1, x2;
+
+   x1 <$ dlist d n1;
+   x2 <$ dlist d n2;
+
+   return x1 ++ x2;
+  }
+}.
+
+equiv sample_samplecat : 
+    Sample.sample ~ SampleX.samplecat :
+    0 <= n1{2} /\ 0 <= n2{2} /\ n{1} = n1{2} + n2{2}
+    ==>
+    ={res}.
+proof.
+bypr (res{1}) (res{2}) => /> &1 &2 l Hn1 Hn2 ->.
+rewrite pr_Sample.
+case: (size l = n1{2} + n2{2}) => El; last first.
+  + rewrite dlist1E 1:/# ifF 1:/#.
+    byphoare (: n1=n1{2} /\ n2=n2{2} ==> res=l) => />.
+    hoare; proc; auto => /> l1.
+    rewrite supp_dlist // => [[Hl1] _] l2.
+    rewrite supp_dlist // => [[Hl2] _].
+    by smt(size_cat).
+byphoare (: n1=n1{2} /\ n2=n2{2} ==> res=l) => />.
+proc; simplify.
+have := cat_take_drop n1{2} l.
+pose l1 := take n1{2} l.
+pose l2 := drop n1{2} l; move => /eq_sym Hl.
+have El1 : size l1 = n1{2} by smt(size_take).
+have El2 : size l2 = n2{2} by smt(size_drop).
+seq 1: (x1 = l1)
+       (mu1 (dlist d n1{2}) l1)
+       (mu1 (dlist d n2{2}) l2)
+       _ 0%r (#pre) => //.
+  + by auto.
+  + by rnd (pred1 l1); auto.
+  + rnd (pred1 l2); auto => /> x.
+    rewrite supp_dlist 1://; move=> [Hx _].
+    by smt(catsI).
+  + hoare; auto => /> &m H1 x.
+    rewrite supp_dlist //; move => [Hx _].
+    smt(eqseq_cat size_cat).
+move => />.
+rewrite Hl (:n1{2}+n2{2}=size (l1++l2)).
+  + rewrite size_cat /#.
+by rewrite dlist_cat1E /#. 
+qed.
+
+end DListProgramX.
