proof/correctness/Correctness_Mem.ec
@@ -74,6 +74,34 @@ conseq memset_zero_ll memset_zero_post.
 auto => />.
 qed.
 
+lemma _memset_nseq : 
+    hoare [
+      M(Syscall).__memset_zero_u8 :
+      true
+      ==>
+      to_list res = nseq 4 W8.zero
+    ].
+proof.
+proc.
+while (
+  0 <= to_uint i <= 4 /\
+  forall (k : int), 0 <= k < to_uint i => a.[k] = W8.zero
+). 
+    + auto => /> &hr *; do split; 1,2:smt(@W64).
+      move => ???. rewrite get_setE #smt:(@W64).
+    + auto => /> &hr; split; [smt() |]. move => ? i???. 
+      have ->: to_uint i = 4 by smt(@W64 pow2_64).
+      move => ?. 
+      apply (eq_from_nth witness); [ rewrite size_to_list size_nseq //= |].
+      rewrite size_to_list => *. 
+      rewrite nth_nseq 1:/# get_to_list /#.
+qed.
+
+lemma memset_nseq : 
+    phoare [ M(Syscall).__memset_zero_u8 : true ==>
+       to_list res = nseq 4 W8.zero] = 1%r
+          by conseq memset_zero_ll _memset_nseq; auto.
+
 lemma load_store  (mem : global_mem_t) (ptr : W64.t) (v : W8.t) :
     loadW8 (storeW8 mem (to_uint ptr) v) (to_uint ptr) = v 
       by rewrite /storeW8 /loadW8 get_setE ifT.
