proof/correctness/Correctness_XMSS.ec
@@ -11,10 +11,12 @@ require import Array4 Array8 Array32 Array64 Array68 Array96 Array132 Array136 A
 require import WArray32 WArray96 WArray136.
 
 require import Correctness_Address Correctness_Mem Correctness_Hash.
-require import Utils.
+require import Utils DistrUtils.
 
 require import BitEncoding.
 (*---*) import BitChunking.
+
+require import Termination.
 
 (*** Treehash kg ***)
 
@@ -23,7 +25,7 @@ lemma treehash_kg_correct :
       M(Syscall).__treehash ~ TreeHash.treehash :
       true
       ==>
-      to_list res{1}.`1 = res{2}.`1 (* we ignore the second part of the result in the proof for kg *)
+      to_list res{1}.`1 = res{2}.`1 
     ].
 proof.
 proc.
@@ -33,44 +35,11 @@ qed.
 
 (*** Key Gen ***)
 
-lemma _memset_nseq : 
-    hoare [
-      M(Syscall).__memset_zero_u8 :
-      true
-      ==>
-      to_list res = nseq 4 W8.zero
-    ].
-proof.
-proc.
-while (
-  0 <= to_uint i <= 4 /\
-  forall (k : int), 0 <= k < to_uint i => a.[k] = W8.zero
-). 
-    + auto => /> &hr *; do split; 1,2:smt(@W64).
-      move => ???. rewrite get_setE #smt:(@W64).
-    + auto => /> &hr; split; [smt() |]. move => ? i???. 
-      have ->: to_uint i = 4 by smt(@W64 pow2_64).
-      move => ?. 
-      apply (eq_from_nth witness); [ rewrite size_to_list size_nseq //= |].
-      rewrite size_to_list => *. 
-      rewrite nth_nseq 1:/# get_to_list /#.
-qed.
+clone import DListProgramX as T
+  with type t <- W8.t,
+       op d <- W8.dword.
 
-require import Termination.
-
-lemma get8_nth (x : W8.t list) (i : int) :
-    0 <= i < 96 =>
-      get8 (WArray96.of_list x) i = nth W8.zero x i.
-proof.
-move => H.
-rewrite /get8 get_of_list; [assumption | trivial].
-qed.
-
-lemma memset_nseq : 
-    phoare [ M(Syscall).__memset_zero_u8 : true ==>
-       to_list res = nseq 4 W8.zero] = 1%r
-          by conseq memset_zero_ll _memset_nseq; auto.
-
+(*** Keygen without OID ***)
 lemma xmss_kg_no_oid : 
     n = XMSS_N /\ 
     d = XMSS_D =>
@@ -78,182 +47,189 @@ lemma xmss_kg_no_oid :
       M(Syscall).__xmssmt_core_keypair ~ XMSS_MT_PRF.kg :
       true 
       ==>
-(*      res{2}.`1 = EncodeSk_NoOID res{1}.`2 /\
-      res{2}.`2 = EncodePk_NoOID res{1}.`1
-*)
-      true
+      res{2}.`1 = EncodeSkNoOID res{1}.`2 /\
+      res{2}.`2 = EncodePkNoOID res{1}.`1
     ].
 proof.
-rewrite /XMSS_N => [#] ??. 
-proc.
-seq 3 2 : (true); first by auto. 
-seq 0 4 : (
-  #pre /\
-  size sk_seed{2}  = n /\
-  size sk_prf{2}   = n /\
-  size pub_seed{2} = n /\
-  size root{2}     = n
-); first by auto => />; rewrite size_nseq /#.
-swap {2} [3..5] -2.
+rewrite /XMSS_N /XMSS_D => [#] *. 
+proc. 
+seq 3 6 : (true); first by auto. 
+swap {2} [3..5] -2. 
 seq 1 3 : (
-  #pre /\
-  to_list seed_p{1} = sk_seed{2} ++ sk_prf{2} ++ pub_seed{2}
+  to_list seed_p{1} = sk_seed{2} ++ sk_prf{2} ++ pub_seed{2} /\
+  size sk_seed{2} = 32 /\
+  size sk_prf{2} = 32 /\
+  size pub_seed{2} = 32 
 ).
-    + inline {1}; wp; sp; auto => />. 
-      rnd{1}. do 3! rnd{2}. skip => /> &2 H0 H1 H2 H3 sk_seed0 ? sk_prf0 T1 pub_seed0? ; split. 
-        - apply dmap_ll. rewrite /darray dmap_ll dlist_ll #smt:(@W8). 
-        - move => ? a0.
-          rewrite /darray dmap_comp /(\o) /get8 => H4.
-          have E0: size sk_seed0 = 32 by smt(@DList).
-          have E1: size sk_prf0 = 32 by smt(@DList). 
-          have E2: size pub_seed0 = 32 by smt(@DList).
-          do split; 1..3:smt().  
-          apply (eq_from_nth witness).
-               +  by rewrite size_to_list !size_cat E0 E1 E2. 
-          move => i. rewrite size_to_list => Hi.
-          rewrite !nth_cat size_cat E0 E1 //=.
-          case (0 <= i < 32).
-             * move => H. rewrite ifT 1:/# ifT 1:/#. admit.          
-          case (32 <= i < 64).
-             * move => H?. rewrite ifT 1:/# ifF 1:/#. admit.
-          move => ??. 
-          have H: 64 <= i < 96 by smt().
-          rewrite ifF 1:/#.                     
-          admit.
-inline {1} M(Syscall).__xmssmt_core_seed_keypair.
-sp 3 0.
-seq 9 0 : (#pre); first by auto. 
+  + inline {1}; wp; sp; auto => />. 
+    transitivity {2} { pub_seed <$ dlist W8.dword 96; }
+    (true ==> to_list a{1} = pub_seed{2})
+    (true ==> pub_seed{1} = (sk_seed{2} ++ sk_prf{2} ++ pub_seed{2}) /\ size sk_seed{2} = 32 /\
+  size sk_prf{2} = 32 /\
+  size pub_seed{2} = 32 ) => //.
+        - rnd Array96.to_list (Array96.of_list W8.zero): *0 *0.
+          auto => />;  split => [l | ?].
+             * rewrite supp_dmap; move => [x].
+               rewrite supp_dlist // => /> E _.
+               by rewrite of_listK.
+          split => [l | ?].
+             * rewrite supp_dmap; move=> [x].                
+               rewrite darray_dlist dmap_comp /(\o) /= supp_dlist //; move=> [[Ex Hx] ->].
+               rewrite dmap_id dmap1E /(\o) /pred1 /=.
+               apply mu_eq_support => y.
+               rewrite supp_dlist //=; move=> [Ey Hy].
+               rewrite eqboolP; split => //.
+               move => E.
+               by rewrite -(Array96.of_listK W8.zero y) // E of_listK.
+          move => a; rewrite darray_dlist dmap_comp supp_dmap.              
+          move => [l]; rewrite supp_dlist // => [[[Esz] H]].
+          rewrite /(\o) /= => ->.
+          by rewrite of_listK //= dmap_id supp_dlist //.
+        (* At this point we're only working with distributions over lists *)
+        - outline {1} [1] { pub_seed <@ T.Program.Sample.sample(96); }.
+          transitivity {1} { pub_seed <@ T.SampleX.samplecat(64,32); }
+          (true ==> ={pub_seed})
+          (true ==> pub_seed{1} = sk_seed{2} ++ sk_prf{2} ++ pub_seed{2} /\ 
+                    size sk_seed{2} = 32 /\ size sk_prf{2} = 32 /\ size pub_seed{2} = 32) => //.
+             * by call sample_samplecat => //.
+          inline*; swap {1} 2 1.
+          seq 2 2: (x1{1} = sk_seed{2} ++ sk_prf{2} /\ size sk_seed{2} = 32 /\ size sk_prf{2} = 32 /\ size pub_seed{2} = 32).
+             * outline {1} [1-2] { x1 <@ T.Program.Sample.sample(64); }.
+               transitivity {1}  { x1 <@ T.SampleX.samplecat(32,32); }
+               (true ==> ={x1})
+               (true ==> x1{1} = sk_seed{2} ++ sk_prf{2} /\ size sk_seed{2} = 32 /\ size sk_prf{2} = 32 /\ size pub_seed{2} = 32) => //.
+                 + by call sample_samplecat => //.
+               inline*; auto; rewrite (: n = 32) //=. 
+             * admit.
+            * admit. 
+(* TODO: FIXME: Add size = 32 to these *)
+seq 0 0 : (#pre /\ size sk_seed{2} = 32 /\ size sk_prf{2} = 32 /\ size pub_seed{2} = 32); first by admit. (* FIXME This should be in the post of the previous seq *) 
+(* TODO: FIXME: Add size = 32 to these *)
+inline {1} M(Syscall).__xmssmt_core_seed_keypair. 
+seq 12 0 : (#pre /\ pk0{1} = pk{1} /\  sk0{1} = sk{1} /\ seed0{1} = seed_p{1}); first by auto. 
 seq 1 1 : (#pre /\ address{2} = top_tree_addr{1}).
-    + inline {1}; wp; sp. 
+    + (* exists * top_tree_addr{1}; elim * => _P; call {1} (zero_addr_op_impl _P). *) (* FIXME: TODO: This should work but I get a invalid goal shape *)
+      inline {1}; wp; sp. 
       while {1} (0 <= i{1} <= 8 /\ forall (k : int), 0 <= k < i{1} => addr0{1}.[k] = W32.zero) (8 - i{1}).
          * auto => /> *; do split;1,2,4:smt(); move => k??; rewrite get_setE /#.
          * skip => /> *; split; [smt() |]; move => *; split; [smt() | move => ????; rewrite /zero_address; smt(@Array8)].
 seq 1 1 : (#pre); first by inline {1}; auto => /> *; rewrite /set_layer_addr /#. 
 seq 2 0 : (#pre /\ to_list idx{1} = nseq 4 W8.zero).
     + call {1} memset_nseq; auto. 
-auto => />. 
 seq 1 0 : (
-  (* #pre without the second /\ *)
-  pk0{1} = pk{1} /\
-  seed0{1} = seed_p{1} /\
-  size sk_seed{2} = n /\
-  size sk_prf{2} = n /\ 
-  size pub_seed{2} = n /\ 
-  size root{2} = n /\
-  to_list seed_p{1} = sk_seed{2} ++ sk_prf{2} ++ pub_seed{2} /\
-  address{2} = top_tree_addr{1} /\
-  to_list idx{1} = nseq 4 W8.zero /\
-
-  forall (k : int), 0 <= k < 4 => sk0{1}.[k] = W8.zero
+                 to_list seed_p{1} = sk_seed{2} ++ sk_prf{2} ++ pub_seed{2} /\
+                 size sk_seed{2} = 32 /\ 
+                 size sk_prf{2} = 32 /\ 
+                 size pub_seed{2} = 32 /\
+                 pk0{1} = pk{1} /\ 
+                 seed0{1} = seed_p{1} /\
+                 address{2} = top_tree_addr{1} /\
+                 to_list idx{1} = nseq 4 W8.zero /\
+                 forall (k : int), 0 <= k < 4 => sk0{1}.[k] = W8.zero
 ).
-    + auto => /> ??????? H *; rewrite initE ifT 1:/#. 
-      auto => />; rewrite ifT 1:/# -get_to_list H nth_nseq 1:/# //. 
+    + auto => /> &1 &2 ???? H. 
+      have E : forall (k : int), 0 <= k < 4 => nth witness (to_list idx{1}) k = W8.zero by apply (nseq_nth (to_list idx{1}) 4 W8.zero);assumption.
+      move => k??; rewrite initiE 1:/#; auto => />; rewrite ifT 1://=.
+      rewrite -get_to_list; apply E => //.
 seq 2 0 : (
-    #pre /\
-    forall (k : int), 0 <= k < 64 => buf1{1}.[k] = seed0{1}.[k]
-); first by auto => /> *; rewrite initE ifT 1:/#; auto => />. 
+  #pre /\
+  forall (k : int), 0 <= k < 64 => buf1{1}.[k] = seed_p{1}.[k]
+); first by auto => /> *; smt(@Array64).
 seq 1 0 : (#pre /\ buf0{1} = buf1{1}); first by ecall {1} (_x_memcpy_u8u8_64_post buf1{1}); skip => />. 
 seq 1 0 : (
   #pre /\ 
   forall (k : int), 0 <= k < 64 => sk0{1}.[4 + k] = seed0{1}.[k]
-).
-    + auto => /> &1 &2 ?????? H0 H1; split; move => ???; rewrite initE ifT 1:/#; auto => />; [rewrite ifF /# | rewrite ifT /#]. 
+); first by auto => /> *; split; move => ???; rewrite initE ifT 1:/#; auto => />; [rewrite ifF /# | rewrite ifT /#]. 
 seq 2 0 : (
-  (* from #pre *)
-  pk0{1} = pk{1} /\
-  seed0{1} = seed_p{1} /\
-  size sk_seed{2} = n /\
-  size sk_prf{2} = n /\
-  size pub_seed{2} = n /\
-  size root{2} = n /\
-  to_list seed_p{1} = sk_seed{2} ++ sk_prf{2} ++ pub_seed{2} /\
-  address{2} = top_tree_addr{1} /\
-  to_list idx{1} = nseq 4 W8.zero /\
-  (forall (k : int), 0 <= k < 4  => sk0{1}.[k] = W8.zero) /\
-  (forall (k : int), 0 <= k < 64 => sk0{1}.[4 + k] = seed0{1}.[k]) /\
-
-  forall (k : int), 0 <= k < 32 => bufn1{1}.[k] = seed0{1}.[64 + k]
-); first by auto => /> *; rewrite initE ifT /#.
+  #pre /\
+  forall (k : int), 0 <= k < 32 => bufn1{1}.[k] = seed_p{1}.[64 + k]
+); first by auto => /> *; smt(@Array32).
 seq 1 0 : (#pre /\ bufn0{1} = bufn1{1}); first by ecall {1} (_x_memcpy_u8u8_post bufn1{1}); skip => />. 
 seq 1 0 : (
     #pre /\
-    forall (k : int), 0 <= k < 32 => sk0{1}.[4 + 3 *32 + k] = seed0{1}.[64 + k]
-).
-    + auto => /> *; do split; move => *; rewrite initE ifT 1:/#; auto => />; [| | rewrite ifT /#]; rewrite ifF /#. 
-seq 2 0 : (
-  (* from #pre *)
-  seed0{1} = seed_p{1} /\
-  size sk_seed{2} = n /\
-  size sk_prf{2} = n /\
-  size pub_seed{2} = n /\
-  size root{2} = n /\
+    forall (k : int), 0 <= k < 32 => sk0{1}.[4 + 3 *32 + k] = seed_p{1}.[64 + k]
+); first by auto => /> *; do split; move => *; rewrite initE ifT 1:/#; auto => />; [| | rewrite ifT /#]; rewrite ifF /#. 
+
+(* -------------------------------------------------------------------------------------------------------------------------------- *)
+(* Cleanup pre *)
+seq 0 0 : (
   to_list seed_p{1} = sk_seed{2} ++ sk_prf{2} ++ pub_seed{2} /\
+  size sk_seed{2} = 32 /\
+  size sk_prf{2} = 32 /\
+  size pub_seed{2} = 32 /\
+  pk0{1} = pk{1} /\
+  seed0{1} = seed_p{1} /\
+  address{2} = top_tree_addr{1} /\
+  to_list idx{1} = nseq 4 W8.zero /\
+        
+
+  (forall (k : int), 0 <= k <  4 => sk0{1}.[k] = W8.zero) /\ (* index *)
+  (forall (k : int), 0 <= k < 64 => sk0{1}.[4 + k] = seed_p{1}.[k]) /\ (* sk seed & sk prf *)
+  (forall (k : int), 0 <= k < 32 => sk0{1}.[4 + 3 * 32 + k] = seed_p{1}.[64 + k]) (* pub seed *)
+); first by auto => />. 
+(* -------------------------------------------------------------------------------------------------------------------------------- *)
+seq 2 0 : (
+  #pre /\
+  (forall (k : int), 0 <= k < 32 => bufn1{1}.[k] = sk0{1}.[100 + k]) 
+); first by auto => /> *; rewrite initiE /#. 
+seq 1 0 : (#pre /\ bufn0{1} = bufn1{1}); first by ecall {1} (_x_memcpy_u8u8_post bufn1{1}); skip => />. 
+seq 1 0 : (
+  (* This is #pre but without the "pk0{1} = pk{1}" and the bufn parts *)
+  to_list seed_p{1} = sk_seed{2} ++ sk_prf{2} ++ pub_seed{2} /\
+  size sk_seed{2} = 32 /\
+  size sk_prf{2} = 32 /\
+  size pub_seed{2} = 32 /\
+  seed0{1} = seed_p{1} /\
   address{2} = top_tree_addr{1} /\
   to_list idx{1} = nseq 4 W8.zero /\
   (forall (k : int), 0 <= k < 4 => sk0{1}.[k] = W8.zero) /\
-  (forall (k : int), 0 <= k < 64 => sk0{1}.[4 + k] = seed0{1}.[k]) /\
-  (forall (k : int), 0 <= k < 32 => sk0{1}.[4 + 3 * 32 + k] = seed0{1}.[64 + k]) /\
+  (forall (k : int), 0 <= k < 64 => sk0{1}.[4 + k] = seed_p{1}.[k]) /\
+  (forall (k : int), 0 <= k < 32 => sk0{1}.[4 + 3 * 32 + k] = seed_p{1}.[64 + k]) /\
 
-
-  (forall (k : int), 0 <= k < 32 => bufn1{1}.[k] = sk0{1}.[4 + 3*32 + k])
-); first by auto => /> *; rewrite initE 1:/#.
-seq 1 0 : (#pre /\ bufn0{1} = bufn1{1}); first by ecall {1} (_x_memcpy_u8u8_post bufn1{1}); skip => />. 
-seq 1 0 : (
+  (* this is new *)
+  (forall (k : int), 0 <= k < 32 => pk0{1}.[32 + k] = sk0{1}.[100 + k])
+); first by auto => &1 &2; move => [#] *; do split; 1..10: assumption; move => k?; rewrite initiE /#. 
+seq 2 0 : (
+  (* buf0 = sk seed /\ buf1 = pub seed *)
   #pre /\
-  forall (k : int), 0 <= k < 32 => pk{1}.[32 + k] = bufn0{1}.[k]
+  (forall (k : int), 0 <= k < 32 => bufn0{1}.[k] = sk0{1}.[4 + k]) /\
+  (forall (k : int), 0 <= k < 32 => bufn1{1}.[k] = pk0{1}.[32 + k])
+); first by auto => /> &1 &2 *; split => *; rewrite initiE //=.
+
+seq 0 1 : (
+  #pre /\
+  toByte sk{2}.`idx 4 = sub sk0{1} 0  4  /\
+  sk{2}.`sk_seed      = sub sk0{1} 4  32 /\
+  sk{2}.`sk_prf       = sub sk0{1} 36 32 /\
+  sk{2}.`pub_seed_sk  = sub sk0{1} 68 32  
 ).
-    + auto => /> &1 &2 ?????? H0 H1 H2 H3 k??. rewrite H3 1:/# H2 1:/#. admit.
+    + auto => /> &1 &2 H0 H1 H2 H3 H4 H5 H6 H7 H8 H9 H10; do split.
+           - rewrite toByteZero. apply (eq_from_nth witness).
+               * rewrite size_nseq size_sub /#.
+             rewrite size_nseq (: max 0 4 = 4) //=  => i Hi.
+             rewrite nth_nseq // nth_sub // /#.
+           - apply (eq_from_nth witness); first by rewrite H1 size_sub //=.
+             rewrite H1 => i Hi. 
+             rewrite nth_sub //= H6 1:/# -get_to_list H0 nth_cat !size_cat H1 H2 ifT 1:/#.
+             rewrite nth_cat H1 ifT 1:/# //=.
+           - apply (eq_from_nth witness); first by rewrite H2 size_sub //=.
+             rewrite H2 => i Hi. 
+             rewrite nth_sub //=.  
+             rewrite (nth_seed_1 (to_list seed_p{1}) sk_seed{2} sk_prf{2} pub_seed{2}) 1:/#.
+             rewrite get_to_list /#. 
+           - apply (eq_from_nth witness); first by rewrite H3 size_sub //=.
+             rewrite H3 => i Hi.
+             rewrite nth_sub 1:/#.
+             rewrite (nth_seed_2 (to_list seed_p{1}) sk_seed{2} sk_prf{2} pub_seed{2}) 1:/#.
+             rewrite get_to_list.  (* Isto esta certo mas a hipotese H7 devia ser falsa *)
+             admit.
+seq 1 1 : (#pre /\ root{2} = to_list root{1}).
+    + admit.
 admit.
 qed.
 
 
-lemma xmss_kg_correct :
-    equiv [
-      M(Syscall).xmss_keypair_jazz ~ XMSS_MT_PRF.kg:
-      true
-      ==>
-      res{2}.`1 = EncodeSk res{1}.`2 /\
-      res{2}.`2 = EncodePk res{1}.`1
-    ].
-proof.
-proc.
-  seq 1 13 : (#post); last by auto.
-seq 0 6 : (
-  size sk_seed{2}  = n /\
-  size sk_prf{2}   = n /\
-  size pub_seed{2} = n
-); first by auto => />; rewrite size_nseq #smt:(ge0_n).  
-inline {1} M(Syscall).__xmss_keypair.
-seq 2 0 : (#pre); first by auto.
-seq 4 0 : (#pre /\ oid{1} = BSWAP_32 W32.one).
-  + auto. 
 
-
-
-
-(* This needs to be changed accordingly *)
-inline M(Syscall).__xmssmt_core_keypair_ M(Syscall)._xmssmt_core_keypair M(Syscall).__xmssmt_core_keypair.
-seq 11 0 : (#pre); first by auto.  (* E possivel que isto esteja errado *)
-seq 0 1 : (#pre /\ address{2} = zero_address); first by auto.
-seq 1 3 : (#pre /\ to_list seed_p{1} = sk_seed{2} ++ sk_prf{2} ++ pub_seed{2}).
-  + inline {1}; sp; auto => />. 
-(*
-    rnd () (Array96.of_list witness).
-    auto => /> *; do split. 
-     - move => ?. rewrite of_listK
-*)
-admit.
-inline  M(Syscall).__xmssmt_core_seed_keypair.
-
-
-
-seq 9 3 : (#pre). (* this pre is wrong *)
-  + admit.
-seq 0 1 : (#pre /\ sk{2} = EncodeSk sk{1}).
-  + admit.
-seq 0 1 : (#post); last by skip. 
-  + admit.
-qed.
 
 (*** L Tree ***)
 
